wip

src/riot/x509/X509.BasicFields.Extension.fst
@@ -1,14 +1,6 @@
 module X509.BasicFields.Extension
 
-open LowParse.Spec.Base
-open LowParse.Spec.Combinators
-
-open ASN1.Base
-open ASN1.Spec
-
 open X509.Base
-
-module B32 = FStar.Bytes
 
 #set-options "--z3rlimit 32 --fuel 0 --ifuel 0"
 
@@ -24,18 +16,6 @@ module B32 = FStar.Bytes
 //     x509_extValue   : OCTET_STRING `inbound_envelop_tag_with_value_of` s }
 
 (* one extension *)
-/// tuple repr
-let x509_extension_t'
-  (#k: parser_kind)
-  (#t: Type0)
-  (#p: parser k t)
-  (oid: datatype_of_asn1_type OID)
-  (s: serializer p)
-= parse_filter_refine (filter_asn1_oid_TLV_of oid)
-  `tuple2`
-  datatype_of_asn1_type BOOLEAN
-  `tuple2`
- (OCTET_STRING `inbound_envelop_tag_with_value_of` s)
 
 // let synth_x509_extension_t
 //   (#k: parser_kind)
@@ -59,23 +39,7 @@ let x509_extension_t'
 // : GTot (x': x509_extension_t' oid s { x == synth_x509_extension_t oid s x' })
 // = (x.x509_extID, x.x509_extCritical), x.x509_extValue
 
-let parse_x509_extension_kind
-= parse_asn1_TLV_kind_of_type OID
-  `and_then_kind`
-  parse_asn1_TLV_kind_of_type BOOLEAN
-  `and_then_kind`
-  parse_asn1_envelop_tag_with_TLV_kind OCTET_STRING
-
-let parse_x509_extension
-  (#k: parser_kind)
-  (#t: Type0)
-  (#p: parser k t)
-  (oid: datatype_of_asn1_type OID)
-  (s: serializer p)
-  (#instance_t: Type0)
-  (f: x509_extension_t' oid s -> GTot instance_t)
-  (prf: unit{synth_injective f})
-: parser parse_x509_extension_kind (instance_t)
+let parse_x509_extension #k #t #p oid s #instance_t f prf
 =
   parse_asn1_oid_TLV_of oid
   `nondep_then`
@@ -87,18 +51,7 @@ let parse_x509_extension
   `parse_synth`
   (prf; f)
 
-let serialize_x509_extension
-  (#k: parser_kind)
-  (#t: Type0)
-  (#p: parser k t)
-  (oid: datatype_of_asn1_type OID)
-  (s: serializer p)
-  (#instance_t: Type0)
-  (f: x509_extension_t' oid s -> GTot instance_t)
-  (g: instance_t -> x509_extension_t' oid s)
-  (prf: unit{ synth_inverse f g /\
-              synth_injective f })
-: serializer (parse_x509_extension oid s f prf)
+let serialize_x509_extension #k #t #p oid s #instance_t f g prf
 =
   serialize_synth
   (* p1 *) (parse_asn1_oid_TLV_of oid
@@ -119,26 +72,7 @@ let serialize_x509_extension
   (* g1 *) (g)
   (* prf*) (prf)
 
-let lemma_serialize_x509_extension_unfold
-  (#k: parser_kind)
-  (#t: Type0)
-  (#p: parser k t)
-  (oid: datatype_of_asn1_type OID)
-  (s: serializer p)
-  (#instance_t: Type0)
-  (f: x509_extension_t' oid s -> GTot instance_t)
-  (g: instance_t -> x509_extension_t' oid s)
-  (prf: unit{ synth_inverse f g /\
-              synth_injective f })
-  (x: instance_t)
-: Lemma (
-  serialize (serialize_x509_extension oid s f g prf) x ==
-  serialize (serialize_asn1_oid_TLV_of oid) (fst (fst (g x)))
-  `Seq.append`
-  serialize (serialize_asn1_TLV_of_type BOOLEAN) (snd (fst (g x)))
-  `Seq.append`
-  serialize (OCTET_STRING `serialize_asn1_envelop_tag_with_TLV` s) (snd (g x))
-)
+let lemma_serialize_x509_extension_unfold #k #t #p oid s #instance_t f g prf x
 = serialize_nondep_then_eq
   (* s1 *) (serialize_asn1_oid_TLV_of oid)
   (* s2 *) (serialize_asn1_TLV_of_type BOOLEAN)
@@ -172,25 +106,7 @@ let lemma_serialize_x509_extension_unfold
   (* in *) x
 
 #push-options "--z3rlimit 32 --fuel 4 --ifuel 4"
-let lemma_serialize_x509_extension_size
-  (#k: parser_kind)
-  (#t: Type0)
-  (#p: parser k t)
-  (oid: datatype_of_asn1_type OID)
-  (s: serializer p)
-  (#instance_t: Type0)
-  (f: x509_extension_t' oid s -> GTot instance_t)
-  (g: instance_t -> x509_extension_t' oid s)
-  (prf: unit{ synth_inverse f g /\
-              synth_injective f })
-  (x: instance_t)
-: Lemma (
-  Seq.length (serialize (serialize_x509_extension oid s f g prf) x) ==
-  length_of_asn1_primitive_TLV #OID (fst (fst (g x))) +
-  length_of_asn1_primitive_TLV #BOOLEAN (snd (fst (g x))) +
-  length_of_TLV OCTET_STRING (length_of_opaque_serialization s (snd (g x))) /\
-  length_of_asn1_primitive_TLV (snd (fst (g x))) == 3
-)
+let lemma_serialize_x509_extension_size #k #t #p oid s #instance_t f g prf x
 = lemma_serialize_x509_extension_unfold oid s f g prf x;
   lemma_serialize_asn1_oid_TLV_of_size oid (fst (fst (g x)));
   lemma_serialize_asn1_envelop_tag_with_TLV_size
@@ -200,90 +116,20 @@ let lemma_serialize_x509_extension_size
   lemma_serialize_asn1_boolean_TLV_size (snd (fst (g x)))
 #pop-options
 
-unfold
-let x509_extension_t_inbound
-  (#k: parser_kind)
-  (#t: Type0)
-  (#p: parser k t)
-  (oid: datatype_of_asn1_type OID)
-  (s: serializer p)
-  (#instance_t: Type0)
-  (f: x509_extension_t' oid s -> GTot instance_t)
-  (g: instance_t -> x509_extension_t' oid s)
-  (prf: unit{ synth_inverse f g /\
-              synth_injective f })
-= inbound_sequence_value_of
-  (* s *) (serialize_x509_extension oid s f g prf)
-
-/// SEQUENCE TLV
-
-let parse_x509_extension_sequence_TLV_kind
-= parse_asn1_envelop_tag_with_TLV_kind SEQUENCE
-
-unfold
-let parse_x509_extension_sequence_TLV
-  (#k: parser_kind)
-  (#t: Type0)
-  (#p: parser k t)
-  (oid: datatype_of_asn1_type OID)
-  (s: serializer p)
-  (#instance_t: Type0)
-  (f: x509_extension_t' oid s -> GTot instance_t)
-  (g: instance_t -> x509_extension_t' oid s)
-  (prf: unit{ synth_inverse f g /\
-              synth_injective f })
-: parser parse_x509_extension_sequence_TLV_kind (x509_extension_t_inbound oid s f g prf)
+let parse_x509_extension_sequence_TLV #k #t #p oid s #instance_t f g prf
 = parse_asn1_sequence_TLV
   (* s *) (serialize_x509_extension oid s f g prf)
 
-unfold
-let serialize_x509_extension_sequence_TLV
-  (#k: parser_kind)
-  (#t: Type0)
-  (#p: parser k t)
-  (oid: datatype_of_asn1_type OID)
-  (s: serializer p)
-  (#instance_t: Type0)
-  (f: x509_extension_t' oid s -> GTot instance_t)
-  (g: instance_t -> x509_extension_t' oid s)
-  (prf: unit{ synth_inverse f g /\
-              synth_injective f })
-: serializer (parse_x509_extension_sequence_TLV oid s f g prf)
+let serialize_x509_extension_sequence_TLV #k #t #p oid s #instance_t f g prf
 = serialize_asn1_sequence_TLV
   (* s *) (serialize_x509_extension oid s f g prf)
 
-unfold
-let lemma_serialize_x509_extension_sequence_TLV_unfold
-  (#k: parser_kind)
-  (#t: Type0)
-  (#p: parser k t)
-  (oid: datatype_of_asn1_type OID)
-  (s: serializer p)
-  (#instance_t: Type0)
-  (f: x509_extension_t' oid s -> GTot instance_t)
-  (g: instance_t -> x509_extension_t' oid s)
-  (prf: unit{ synth_inverse f g /\
-              synth_injective f })
-  (x: x509_extension_t_inbound oid s f g prf)
-: Lemma ( predicate_serialize_asn1_sequence_TLV_unfold (serialize_x509_extension oid s f g prf) x )
+let lemma_serialize_x509_extension_sequence_TLV_unfold #k #t #p oid s #instance_t f g prf x
 = lemma_serialize_asn1_sequence_TLV_unfold
   (* s *) (serialize_x509_extension oid s f g prf)
   x
 
-unfold
-let lemma_serialize_x509_extension_sequence_TLV_size
-  (#k: parser_kind)
-  (#t: Type0)
-  (#p: parser k t)
-  (oid: datatype_of_asn1_type OID)
-  (s: serializer p)
-  (#instance_t: Type0)
-  (f: x509_extension_t' oid s -> GTot instance_t)
-  (g: instance_t -> x509_extension_t' oid s)
-  (prf: unit{ synth_inverse f g /\
-              synth_injective f })
-  (x: x509_extension_t_inbound oid s f g prf)
-: Lemma ( predicate_serialize_asn1_sequence_TLV_size (serialize_x509_extension oid s f g prf) x )
+let lemma_serialize_x509_extension_sequence_TLV_size #k #t #p oid s #instance_t f g prf x
 = lemma_serialize_asn1_sequence_TLV_size
   (* s *) (serialize_x509_extension oid s f g prf)
   x
@@ -302,21 +148,7 @@ open ASN1.Low
 // = (x.x509_extID, x.x509_extCritical), x.x509_extValue
 
 //AR: 06/11: this and the next one seem helpers to me?
-inline_for_extraction noextract
-let serialize32_x509_extension_backwards
-  (#k: parser_kind)
-  (#t: Type0)
-  (#p: parser k t)
-  (#s: serializer p)
-  (oid: datatype_of_asn1_type OID)
-  (s32: serializer32_backwards s)
-  (#instance_t: Type0)
-  (f: x509_extension_t' oid s -> GTot instance_t)
-  (g: instance_t -> x509_extension_t' oid s)
-  (g': (x2: instance_t) -> Tot (x1: x509_extension_t' oid s { x1 == g x2 }))
-  (prf: unit{ synth_inverse f g /\
-              synth_injective f })
-: serializer32_backwards (serialize_x509_extension oid s f g prf)
+let serialize32_x509_extension_backwards #k #t #p #s oid s32 #instance_t f g g' prf
 = serialize32_synth_backwards
   (* s32*) (serialize32_asn1_oid_TLV_of_backwards oid
             `serialize32_nondep_then_backwards`
@@ -330,20 +162,6 @@ let serialize32_x509_extension_backwards
   (* g1'*) (g')
   (* prf*) (prf)
 
-inline_for_extraction noextract
-let serialize32_x509_extension_sequence_TLV_backwards
-  (#k: parser_kind)
-  (#t: Type0)
-  (#p: parser k t)
-  (#s: serializer p)
-  (oid: datatype_of_asn1_type OID)
-  (s32: serializer32_backwards s)
-  (#instance_t: Type0)
-  (f: x509_extension_t' oid s -> GTot instance_t)
-  (g: instance_t -> x509_extension_t' oid s)
-  (g': (x2: instance_t) -> Tot (x1: x509_extension_t' oid s { x1 == g x2 }))
-  (prf: unit{ synth_inverse f g /\
-              synth_injective f })
-: serializer32_backwards (serialize_x509_extension_sequence_TLV oid s f g prf)
+let serialize32_x509_extension_sequence_TLV_backwards #k #t #p #s oid s32 #instance_t f g g' prf
 = serialize32_asn1_sequence_TLV_backwards
   (* s32 *) (serialize32_x509_extension_backwards oid s32 f g g' prf)
