src/riot/x509/X509.BasicFields.Extension.fsti
@@ -1,0 +1,248 @@
+module X509.BasicFields.Extension
+
+open ASN1.Spec
+
+open X509.Base
+
+// inline_for_extraction
+// type x509_extension_t
+//   (#k: parser_kind)
+//   (#t: Type0)
+//   (#p: parser k t)
+//   (oid: datatype_of_asn1_type OID)
+//   (s: serializer p)
+// = { x509_extID      : x:datatype_of_asn1_type OID {x == oid};
+//     x509_extCritical: datatype_of_asn1_type BOOLEAN;
+//     x509_extValue   : OCTET_STRING `inbound_envelop_tag_with_value_of` s }
+
+(* one extension *)
+/// tuple repr
+let x509_extension_t'
+  (#k: parser_kind)
+  (#t: Type0)
+  (#p: parser k t)
+  (oid: datatype_of_asn1_type OID)
+  (s: serializer p)
+= parse_filter_refine (filter_asn1_oid_TLV_of oid)
+  `tuple2`
+  datatype_of_asn1_type BOOLEAN
+  `tuple2`
+ (OCTET_STRING `inbound_envelop_tag_with_value_of` s)
+
+// let synth_x509_extension_t
+//   (#k: parser_kind)
+//   (#t: Type0)
+//   (#p: parser k t)
+//   (oid: datatype_of_asn1_type OID)
+//   (s: serializer p)
+//   (x': x509_extension_t' oid s)
+// : GTot (x509_extension_t oid s)
+// = { x509_extID       = fst (fst x');
+//     x509_extCritical = snd (fst x');
+//     x509_extValue    = snd x' }
+
+// let synth_x509_extension_t'
+//   (#k: parser_kind)
+//   (#t: Type0)
+//   (#p: parser k t)
+//   (oid: datatype_of_asn1_type OID)
+//   (s: serializer p)
+//   (x: x509_extension_t oid s)
+// : GTot (x': x509_extension_t' oid s { x == synth_x509_extension_t oid s x' })
+// = (x.x509_extID, x.x509_extCritical), x.x509_extValue
+
+inline_for_extraction noextract
+let parse_x509_extension_kind
+= parse_asn1_TLV_kind_of_type OID
+  `and_then_kind`
+  parse_asn1_TLV_kind_of_type BOOLEAN
+  `and_then_kind`
+  parse_asn1_envelop_tag_with_TLV_kind OCTET_STRING
+
+val parse_x509_extension
+  (#k: parser_kind)
+  (#t: Type0)
+  (#p: parser k t)
+  (oid: datatype_of_asn1_type OID)
+  (s: serializer p)
+  (#instance_t: Type0)
+  (f: x509_extension_t' oid s -> GTot instance_t)
+  (prf: unit{synth_injective f})
+: parser parse_x509_extension_kind (instance_t)
+
+val serialize_x509_extension
+  (#k: parser_kind)
+  (#t: Type0)
+  (#p: parser k t)
+  (oid: datatype_of_asn1_type OID)
+  (s: serializer p)
+  (#instance_t: Type0)
+  (f: x509_extension_t' oid s -> GTot instance_t)
+  (g: instance_t -> x509_extension_t' oid s)
+  (prf: unit{ synth_inverse f g /\
+              synth_injective f })
+: serializer (parse_x509_extension oid s f prf)
+
+val lemma_serialize_x509_extension_unfold
+  (#k: parser_kind)
+  (#t: Type0)
+  (#p: parser k t)
+  (oid: datatype_of_asn1_type OID)
+  (s: serializer p)
+  (#instance_t: Type0)
+  (f: x509_extension_t' oid s -> GTot instance_t)
+  (g: instance_t -> x509_extension_t' oid s)
+  (prf: unit{ synth_inverse f g /\
+              synth_injective f })
+  (x: instance_t)
+: Lemma (
+  serialize (serialize_x509_extension oid s f g prf) x ==
+  serialize (serialize_asn1_oid_TLV_of oid) (fst (fst (g x)))
+  `Seq.append`
+  serialize (serialize_asn1_TLV_of_type BOOLEAN) (snd (fst (g x)))
+  `Seq.append`
+  serialize (OCTET_STRING `serialize_asn1_envelop_tag_with_TLV` s) (snd (g x))
+)
+
+val lemma_serialize_x509_extension_size
+  (#k: parser_kind)
+  (#t: Type0)
+  (#p: parser k t)
+  (oid: datatype_of_asn1_type OID)
+  (s: serializer p)
+  (#instance_t: Type0)
+  (f: x509_extension_t' oid s -> GTot instance_t)
+  (g: instance_t -> x509_extension_t' oid s)
+  (prf: unit{ synth_inverse f g /\
+              synth_injective f })
+  (x: instance_t)
+: Lemma (
+  Seq.length (serialize (serialize_x509_extension oid s f g prf) x) ==
+  length_of_asn1_primitive_TLV #OID (fst (fst (g x))) +
+  length_of_asn1_primitive_TLV #BOOLEAN (snd (fst (g x))) +
+  length_of_TLV OCTET_STRING (length_of_opaque_serialization s (snd (g x))) /\
+  length_of_asn1_primitive_TLV (snd (fst (g x))) == 3
+)
+
+unfold
+let x509_extension_t_inbound
+  (#k: parser_kind)
+  (#t: Type0)
+  (#p: parser k t)
+  (oid: datatype_of_asn1_type OID)
+  (s: serializer p)
+  (#instance_t: Type0)
+  (f: x509_extension_t' oid s -> GTot instance_t)
+  (g: instance_t -> x509_extension_t' oid s)
+  (prf: unit{ synth_inverse f g /\
+              synth_injective f })
+= inbound_sequence_value_of
+  (* s *) (serialize_x509_extension oid s f g prf)
+
+/// SEQUENCE TLV
+
+inline_for_extraction noextract
+let parse_x509_extension_sequence_TLV_kind
+= parse_asn1_envelop_tag_with_TLV_kind SEQUENCE
+
+inline_for_extraction noextract
+val parse_x509_extension_sequence_TLV
+  (#k: parser_kind)
+  (#t: Type0)
+  (#p: parser k t)
+  (oid: datatype_of_asn1_type OID)
+  (s: serializer p)
+  (#instance_t: Type0)
+  (f: x509_extension_t' oid s -> GTot instance_t)
+  (g: instance_t -> x509_extension_t' oid s)
+  (prf: unit{ synth_inverse f g /\
+              synth_injective f })
+: parser parse_x509_extension_sequence_TLV_kind (x509_extension_t_inbound oid s f g prf)
+
+inline_for_extraction noextract
+val serialize_x509_extension_sequence_TLV
+  (#k: parser_kind)
+  (#t: Type0)
+  (#p: parser k t)
+  (oid: datatype_of_asn1_type OID)
+  (s: serializer p)
+  (#instance_t: Type0)
+  (f: x509_extension_t' oid s -> GTot instance_t)
+  (g: instance_t -> x509_extension_t' oid s)
+  (prf: unit{ synth_inverse f g /\
+              synth_injective f })
+: serializer (parse_x509_extension_sequence_TLV oid s f g prf)
+
+val lemma_serialize_x509_extension_sequence_TLV_unfold
+  (#k: parser_kind)
+  (#t: Type0)
+  (#p: parser k t)
+  (oid: datatype_of_asn1_type OID)
+  (s: serializer p)
+  (#instance_t: Type0)
+  (f: x509_extension_t' oid s -> GTot instance_t)
+  (g: instance_t -> x509_extension_t' oid s)
+  (prf: unit{ synth_inverse f g /\
+              synth_injective f })
+  (x: x509_extension_t_inbound oid s f g prf)
+: Lemma ( predicate_serialize_asn1_sequence_TLV_unfold (serialize_x509_extension oid s f g prf) x )
+
+val lemma_serialize_x509_extension_sequence_TLV_size
+  (#k: parser_kind)
+  (#t: Type0)
+  (#p: parser k t)
+  (oid: datatype_of_asn1_type OID)
+  (s: serializer p)
+  (#instance_t: Type0)
+  (f: x509_extension_t' oid s -> GTot instance_t)
+  (g: instance_t -> x509_extension_t' oid s)
+  (prf: unit{ synth_inverse f g /\
+              synth_injective f })
+  (x: x509_extension_t_inbound oid s f g prf)
+: Lemma ( predicate_serialize_asn1_sequence_TLV_size (serialize_x509_extension oid s f g prf) x )
+
+open ASN1.Low
+
+// inline_for_extraction noextract
+// let synth_x509_extension_t'_impl
+//   (#k: parser_kind)
+//   (#t: Type0)
+//   (#p: parser k t)
+//   (oid: datatype_of_asn1_type OID)
+//   (s: serializer p)
+//   (x: x509_extension_t oid s)
+// : Tot (x': x509_extension_t' oid s { x' == synth_x509_extension_t' oid s x })
+// = (x.x509_extID, x.x509_extCritical), x.x509_extValue
+
+//AR: 06/11: this and the next one seem helpers to me?
+inline_for_extraction noextract
+val serialize32_x509_extension_backwards
+  (#k: parser_kind)
+  (#t: Type0)
+  (#p: parser k t)
+  (#s: serializer p)
+  (oid: datatype_of_asn1_type OID)
+  (s32: serializer32_backwards s)
+  (#instance_t: Type0)
+  (f: x509_extension_t' oid s -> GTot instance_t)
+  (g: instance_t -> x509_extension_t' oid s)
+  (g': (x2: instance_t) -> Tot (x1: x509_extension_t' oid s { x1 == g x2 }))
+  (prf: unit{ synth_inverse f g /\
+              synth_injective f })
+: serializer32_backwards (serialize_x509_extension oid s f g prf)
+
+inline_for_extraction noextract
+val serialize32_x509_extension_sequence_TLV_backwards
+  (#k: parser_kind)
+  (#t: Type0)
+  (#p: parser k t)
+  (#s: serializer p)
+  (oid: datatype_of_asn1_type OID)
+  (s32: serializer32_backwards s)
+  (#instance_t: Type0)
+  (f: x509_extension_t' oid s -> GTot instance_t)
+  (g: instance_t -> x509_extension_t' oid s)
+  (g': (x2: instance_t) -> Tot (x1: x509_extension_t' oid s { x1 == g x2 }))
+  (prf: unit{ synth_inverse f g /\
+              synth_injective f })
+: serializer32_backwards (serialize_x509_extension_sequence_TLV oid s f g prf)
